theories/Symbolic/Propositions.v
@@ -1796,9 +1796,9 @@ Module Type SymPropOn
     | eterm_relval  (σ : Ty) (v : RelVal σ) : ETerm σ
     | eterm_binop   {σ1 σ2 σ3} (op : BinOp σ1 σ2 σ3) (t1 : ETerm σ1) (t2 : ETerm σ2) : ETerm σ3
     | eterm_unop    {σ1 σ2} (op : UnOp σ1 σ2) (t : ETerm σ1) : ETerm σ2
-    (* | eterm_tuple   {σs : Ctx Ty} (ts : Env ETerm σs) : ETerm (ty.tuple σs) *)
+    | eterm_tuple   {σs : Ctx Ty} (ts : Env ETerm σs) : ETerm (ty.tuple σs)
     | eterm_union   {U : unioni} (K : unionk U) (t : ETerm (unionk_ty U K)) : ETerm (ty.union U)
-    (* | eterm_record  (R : recordi) (ts : NamedEnv ETerm (recordf_ty R)) : ETerm (ty.record R) *)
+    | eterm_record  (R : recordi) (ts : NamedEnv ETerm (recordf_ty R)) : ETerm (ty.record R)
     .
     Global Arguments eterm_relval σ v : clear implicits.
 
@@ -1856,9 +1856,9 @@ Module Type SymPropOn
         | term_relval σ v             => eterm_relval σ v
         | term_binop op t1 t2         => eterm_binop op (erase t1) (erase t2)
         | term_unop op t              => eterm_unop op (erase t)
-        (* | term_tuple ts              => eterm_tuple (env.map (fun _ => erase) ts) *)
+        | term_tuple ts              => eterm_tuple (env.map (fun _ => erase) ts)
         | term_union U K t           => eterm_union K (erase t)
-        (* | term_record R ts           => eterm_record R (env.map (fun _ => erase) ts) *)
+        | term_record R ts           => eterm_record R (env.map (fun _ => erase) ts)
         end.
 
     Definition erase_formula {Σ} : Formula Σ -> EFormula :=
@@ -1932,8 +1932,8 @@ Module Type SymPropOn
 
     Import option.notations.
 
-    Definition inst_env' (ι : list { σ : Ty & Val σ}) (inst_eterm : forall τ, ETerm τ -> option (Val τ)) :
-      forall {Δ : Ctx Ty}, Env ETerm Δ -> option (Env Val Δ) :=
+    Definition inst_env' (ι : list { σ : Ty & RelVal σ}) (inst_eterm : forall τ, ETerm τ -> option (RelVal τ)) :
+      forall {Δ : Ctx Ty}, Env ETerm Δ -> option (Env RelVal Δ) :=
        fix inst_env {Δ} E :=
          match E with
          | [] => Some []
@@ -1971,13 +1971,13 @@ Module Type SymPropOn
             Some (bop.evalRel op v1 v2)
         | @eterm_unop σ1 σ2 op t0  =>
             uop.evalRel op <$> inst_eterm t0
-        (* | @eterm_tuple σs ts => *)
-        (*     envrec.of_env (σs := σs) <$> inst_env' ι inst_eterm ts *)
+        | @eterm_tuple σs ts =>
+            ty.envToRelValTuple (Γ := σs) <$> inst_env' ι inst_eterm ts
         | @eterm_union U K t0 =>
             rv <- inst_eterm t0 ;;
             Some (ty.unionv_fold_rel U (existT K rv))
-        (* | @eterm_record R ts => *)
-        (*     recordv_fold R <$> inst_namedenv' ι inst_eterm ts *)
+        | @eterm_record R ts =>
+            ty.recordv_fold_rel R <$> inst_namedenv' ι inst_eterm ts
         end.
 
     Definition inst_namedenv (ι : list { σ : Ty & RelVal σ}) {N} {Δ : NCtx N Ty} :
@@ -2112,15 +2112,15 @@ Module Type SymPropOn
       - reflexivity.
       - now rewrite IHt1, IHt2.
       - now rewrite IHt.
-      (* - cbn. apply option.map_eq_some. *)
-      (*   induction IH as [|Δ E σ t _ IHE IHt]; cbn in *. *)
-      (*   + reflexivity. *)
-      (*   + now rewrite IHt, IHE. *)
+      - cbn. apply option.map_eq_some.
+        induction IH as [|Δ E σ t _ IHE IHt]; cbn in *.
+        + reflexivity.
+        + now rewrite IHt, IHE.
       - now rewrite IHt.
-      (* - cbn. apply option.map_eq_some. *)
-      (*   induction IH as [|Δ E [x σ] t _ IHE IHt]; cbn in *. *)
-      (*   + reflexivity. *)
-      (*   + now rewrite IHt, IHE. *)
+      - cbn. apply option.map_eq_some.
+        induction IH as [|Δ E [x σ] t _ IHE IHt]; cbn in *.
+        + reflexivity.
+        + now rewrite IHt, IHE.
     Qed.
 
     Lemma inst_env_erase {Σ Δ} (ts : Env (Term Σ) Δ) (ι : Valuation Σ) :
