theories/Syntax/Terms.v
@@ -64,16 +64,16 @@ Module Type TermsOn (Import TY : Types).
   | term_relval  (σ : Ty) : RelVal σ → Term Σ σ
   | term_binop   {σ1 σ2 σ3} (op : BinOp σ1 σ2 σ3) (t1 : Term Σ σ1) (t2 : Term Σ σ2) : Term Σ σ3
   | term_unop    {σ1 σ2} (op : UnOp σ1 σ2) (t : Term Σ σ1) : Term Σ σ2
-  (* | term_tuple   {σs} (ts : Env (Term Σ) σs) : Term Σ (ty.tuple σs) *)
+  | term_tuple   {σs} (ts : Env (Term Σ) σs) : Term Σ (ty.tuple σs)
   | term_union   {U : unioni} (K : unionk U) (t : Term Σ (unionk_ty U K)) : Term Σ (ty.union U)
-  (* | term_record  (R : recordi) (ts : NamedEnv (Term Σ) (recordf_ty R)) : Term Σ (ty.record R) *)
+  | term_record  (R : recordi) (ts : NamedEnv (Term Σ) (recordf_ty R)) : Term Σ (ty.record R)
   .
   #[global] Arguments term_var {_} _ {_ _}.
   #[global] Arguments term_val {_} _ _.
   #[global] Arguments term_relval {_} _ _.
-  (* #[global] Arguments term_tuple {_ _} ts. *)
+  #[global] Arguments term_tuple {_ _} ts.
   #[global] Arguments term_union {_} U K t.
-  (* #[global] Arguments term_record {_} R ts. *)
+  #[global] Arguments term_record {_} R ts.
   Bind Scope term_scope with Term.
   Derive NoConfusion Signature for Term.
 
@@ -88,8 +88,8 @@ Module Type TermsOn (Import TY : Types).
   Notation term_and := (term_binop bop.and).
   Notation term_or := (term_binop bop.or).
   Notation term_pair := (term_binop bop.pair).
-  (* Notation term_cons := (term_binop bop.cons). *)
-  (* Notation term_append := (term_binop bop.append). *)
+  Notation term_cons := (term_binop bop.cons).
+  Notation term_append := (term_binop bop.append).
   Notation term_shiftr := (term_binop bop.shiftr).
   Notation term_shiftl := (term_binop bop.shiftl).
   Notation term_bvadd := (term_binop bop.bvadd).
@@ -112,11 +112,11 @@ Module Type TermsOn (Import TY : Types).
   Notation term_bvult := (term_binop (bop.relop bop.bvult)).
 
   (* UnOp *)
-  (* Notation term_inl := (term_unop uop.inl). *)
-  (* Notation term_inr := (term_unop uop.inr). *)
+  Notation term_inl := (term_unop uop.inl).
+  Notation term_inr := (term_unop uop.inr).
   Notation term_neg := (term_unop uop.neg).
   Notation term_not := (term_unop uop.not).
-  (* Notation term_rev := (term_unop uop.rev). *)
+  Notation term_rev := (term_unop uop.rev).
   Notation term_sext := (term_unop uop.sext).
   Notation term_zext := (term_unop uop.zext).
   Notation term_get_slice_int := (term_unop uop.get_slice_int).
@@ -129,15 +129,15 @@ Module Type TermsOn (Import TY : Types).
 
   Section DerivedConstructions.
 
-    (* Definition term_enum {Σ} (E : enumi) (k : enumt E) : Term Σ (ty.enum E) := *)
-    (*   term_val (ty.enum E) k. *)
-    (* #[global] Arguments term_enum {_} _ _. *)
+    Definition term_enum {Σ} (E : enumi) (k : enumt E) : Term Σ (ty.enum E) :=
+      term_val (ty.enum E) k.
+    #[global] Arguments term_enum {_} _ _.
 
-    (* Fixpoint term_list {Σ σ} (ts : list (Term Σ σ)) : Term Σ (ty.list σ) := *)
-    (*   match ts with *)
-    (*   | nil       => term_val (ty.list σ) nil *)
-    (*   | cons t ts => term_cons t (term_list ts) *)
-    (*   end. *)
+    Fixpoint term_list {Σ σ} (ts : list (Term Σ σ)) : Term Σ (ty.list σ) :=
+      match ts with
+      | nil       => term_val (ty.list σ) nil
+      | cons t ts => term_cons t (term_list ts)
+      end.
 
     Fixpoint term_bvec {Σ n} (ts : Vector.t (Term Σ ty.bool) n) : Term Σ (ty.bvec n) :=
       match ts with
@@ -188,8 +188,8 @@ Module Type TermsOn (Import TY : Types).
 
     Let PE : ∀ (σs : Ctx Ty), Env (Term Σ) σs → Type :=
       fun σs es => env.All P es.
-    (* Let PNE : ∀ (σs : NCtx recordf Ty), NamedEnv (Term Σ) σs → Type := *)
-    (*   fun σs es => env.All (fun b t => P t) es. *)
+    Let PNE : ∀ (σs : NCtx recordf Ty), NamedEnv (Term Σ) σs → Type :=
+      fun σs es => env.All (fun b t => P t) es.
 
     Hypothesis (pvar : ∀ (l : LVar) (σ : Ty) (lIn : l∷σ ∈ Σ), P (term_var l)).
     Hypothesis (pval : ∀ [σ] (v : Val σ), P (term_val σ v)).
@@ -199,12 +199,12 @@ Module Type TermsOn (Import TY : Types).
                             P t1 → P t2 → P (term_binop op t1 t2))).
     Hypothesis (punop : (∀ [σ1 σ2] (op : UnOp σ1 σ2) (t : Term Σ σ1),
                            P t → P (term_unop op t))).
-    (* Hypothesis (ptuple : (∀ [σs] (ts : Env (Term Σ) σs) (IH : PE ts), *)
-    (*                         P (term_tuple ts))). *)
+    Hypothesis (ptuple : (∀ [σs] (ts : Env (Term Σ) σs) (IH : PE ts),
+                            P (term_tuple ts))).
     Hypothesis (punion : (∀ [U] (K : unionk U) (t : Term Σ (unionk_ty U K)),
                             P t → P (term_union U K t))).
-    (* Hypothesis (precord : (∀ [R] (ts : NamedEnv (Term Σ) (recordf_ty R)) *)
-    (*                          (IH : PNE ts), P (term_record R ts))). *)
+    Hypothesis (precord : (∀ [R] (ts : NamedEnv (Term Σ) (recordf_ty R))
+                             (IH : PNE ts), P (term_record R ts))).
 
     Fixpoint Term_rect [σ] (t : Term Σ σ) {struct t} : P t :=
       match t with
@@ -213,10 +213,10 @@ Module Type TermsOn (Import TY : Types).
       | term_relval σ v     => prelval v
       | term_binop op t1 t2 => pbinop op (Term_rect t1) (Term_rect t2)
       | term_unop op t      => punop op (Term_rect t)
-      (* | term_tuple ts       => ptuple (env.all_intro Term_rect ts) *)
+      | term_tuple ts       => ptuple (env.all_intro Term_rect ts)
       | term_union U K t    => punion K (Term_rect t)
-      (* | term_record R ts    => *)
-      (*     precord (env.all_intro (fun b => Term_rect (σ := type b)) ts) *)
+      | term_record R ts    =>
+          precord (env.all_intro (fun b => Term_rect (σ := type b)) ts)
       end.
 
   End Term_rect.
@@ -333,20 +333,22 @@ Module Type TermsOn (Import TY : Types).
 
   Section Term_list_case.
 
-    (* Context {Σ σ} (P : Term Σ (ty.list σ) → Type). *)
+    Context {Σ σ} (P : Term Σ (ty.list σ) → Type).
 
-    (* Hypothesis (pvar : ∀ (l : LVar) (lIn : l∷ty.list σ ∈ Σ), P (term_var l)). *)
-    (* Hypothesis (pval : ∀ (v : Val (ty.list σ)), P (term_val (ty.list σ) v)). *)
-    (* Hypothesis (pcons : ∀ (t1 : Term Σ σ) (t2 : Term Σ (ty.list σ)), P (term_binop bop.cons t1 t2)). *)
-    (* Hypothesis (pappend : ∀ (t1 : Term Σ (ty.list σ)) (t2 : Term Σ (ty.list σ)), P (term_binop bop.append t1 t2)). *)
-    (* Hypothesis (prev : ∀ (t : Term Σ (ty.list σ)), P (term_unop uop.rev t)). *)
+    Hypothesis (pvar : ∀ (l : LVar) (lIn : l∷ty.list σ ∈ Σ), P (term_var l)).
+    Hypothesis (pval : ∀ (v : Val (ty.list σ)), P (term_val (ty.list σ) v)).
+    Hypothesis (prelval : ∀ (rv : RelVal (ty.list σ)), P (term_relval (ty.list σ) rv)).
+    Hypothesis (pcons : ∀ (t1 : Term Σ σ) (t2 : Term Σ (ty.list σ)), P (term_binop bop.cons t1 t2)).
+    Hypothesis (pappend : ∀ (t1 : Term Σ (ty.list σ)) (t2 : Term Σ (ty.list σ)), P (term_binop bop.append t1 t2)).
+    Hypothesis (prev : ∀ (t : Term Σ (ty.list σ)), P (term_unop uop.rev t)).
 
-    (* Equations(noeqns) Term_list_case (t : Term Σ (ty.list σ)) : P t := *)
-    (* | term_var_in lIn             => pvar lIn *)
-    (* | term_val _ v                => pval v *)
-    (* | term_binop bop.cons t1 t2   => pcons t1 t2 *)
-    (* | term_binop bop.append t1 t2 => pappend t1 t2 *)
-    (* | term_unop uop.rev t         => prev t. *)
+    Equations(noeqns) Term_list_case (t : Term Σ (ty.list σ)) : P t :=
+    | term_var_in lIn             => pvar lIn
+    | term_val _ v                => pval v
+    | term_relval _ rv             => prelval rv
+    | term_binop bop.cons t1 t2   => pcons t1 t2
+    | term_binop bop.append t1 t2 => pappend t1 t2
+    | term_unop uop.rev t         => prev t.
 
   End Term_list_case.
 
@@ -369,18 +371,20 @@ Module Type TermsOn (Import TY : Types).
 
   Section Term_sum_case.
 
-    (* Context {Σ σ1 σ2} (P : Term Σ (ty.sum σ1 σ2) → Type). *)
+    Context {Σ σ1 σ2} (P : Term Σ (ty.sum σ1 σ2) → Type).
 
-    (* Hypothesis (pvar : ∀ (ς : LVar) (ςInΣ : ς∷ty.sum σ1 σ2 ∈ Σ), P (term_var ς)). *)
-    (* Hypothesis (pval : ∀ (v : Val (ty.sum σ1 σ2)), P (term_val (ty.sum σ1 σ2) v)). *)
-    (* Hypothesis (pinl : ∀ (t1 : Term Σ σ1), P (term_unop uop.inl t1)). *)
-    (* Hypothesis (pinr : ∀ (t2 : Term Σ σ2), P (term_unop uop.inr t2)). *)
+    Hypothesis (pvar : ∀ (ς : LVar) (ςInΣ : ς∷ty.sum σ1 σ2 ∈ Σ), P (term_var ς)).
+    Hypothesis (pval : ∀ (v : Val (ty.sum σ1 σ2)), P (term_val (ty.sum σ1 σ2) v)).
+    Hypothesis (prelval : ∀ (rv : RelVal (ty.sum σ1 σ2)), P (term_relval (ty.sum σ1 σ2) rv)).
+    Hypothesis (pinl : ∀ (t1 : Term Σ σ1), P (term_unop uop.inl t1)).
+    Hypothesis (pinr : ∀ (t2 : Term Σ σ2), P (term_unop uop.inr t2)).
 
-    (* Equations(noeqns) Term_sum_case (t : Term Σ (ty.sum σ1 σ2)) : P t := *)
-    (* | term_var_in lIn     => pvar lIn *)
-    (* | term_val _ v        => pval v *)
-    (* | term_unop uop.inl t => pinl t *)
-    (* | term_unop uop.inr t => pinr t. *)
+    Equations(noeqns) Term_sum_case (t : Term Σ (ty.sum σ1 σ2)) : P t :=
+    | term_var_in lIn     => pvar lIn
+    | term_val _ v        => pval v
+    | term_relval _ v     => prelval v
+    | term_unop uop.inl t => pinl t
+    | term_unop uop.inr t => pinr t.
 
   End Term_sum_case.
 
@@ -505,16 +509,18 @@ Module Type TermsOn (Import TY : Types).
 
   Section Term_tuple_case.
 
-    (* Context {Σ σs} (P : Term Σ (ty.tuple σs) → Type). *)
+    Context {Σ σs} (P : Term Σ (ty.tuple σs) → Type).
 
-    (* Hypothesis (pvar : ∀ (l : LVar) (lIn : l∷ty.tuple σs ∈ Σ), P (term_var l)). *)
-    (* Hypothesis (pval : ∀ (v : Val (ty.tuple σs)), P (term_val (ty.tuple σs) v)). *)
-    (* Hypothesis (ptuple : ∀ (ts : Env (Term Σ) σs), P (term_tuple ts)). *)
+    Hypothesis (pvar : ∀ (l : LVar) (lIn : l∷ty.tuple σs ∈ Σ), P (term_var l)).
+    Hypothesis (pval : ∀ (v : Val (ty.tuple σs)), P (term_val (ty.tuple σs) v)).
+    Hypothesis (prelval : ∀ (rv : RelVal (ty.tuple σs)), P (term_relval (ty.tuple σs) rv)).
+    Hypothesis (ptuple : ∀ (ts : Env (Term Σ) σs), P (term_tuple ts)).
 
-    (* Equations(noeqns) Term_tuple_case (t : Term Σ (ty.tuple σs)) : P t := *)
-    (* | term_var_in lIn => pvar lIn *)
-    (* | term_val _ v    => pval v *)
-    (* | term_tuple ts   => ptuple ts. *)
+    Equations(noeqns) Term_tuple_case (t : Term Σ (ty.tuple σs)) : P t :=
+    | term_var_in lIn => pvar lIn
+    | term_val _ v    => pval v
+    | term_relval _ v => prelval v
+    | term_tuple ts   => ptuple ts.
 
   End Term_tuple_case.
 
@@ -537,16 +543,18 @@ Module Type TermsOn (Import TY : Types).
 
   Section Term_record_case.
 
-    (* Context {Σ R} (P : Term Σ (ty.record R) → Type). *)
+    Context {Σ R} (P : Term Σ (ty.record R) → Type).
 
-    (* Variable (pvar : ∀ (l : LVar) (lIn : l∷ty.record R ∈ Σ), P (term_var l)). *)
-    (* Variable (pval : ∀ (v : Val (ty.record R)), P (term_val (ty.record R) v)). *)
-    (* Variable (precord : ∀ (ts : NamedEnv (Term Σ) (recordf_ty R)), P (term_record R ts)). *)
+    Variable (pvar : ∀ (l : LVar) (lIn : l∷ty.record R ∈ Σ), P (term_var l)).
+    Variable (pval : ∀ (v : Val (ty.record R)), P (term_val (ty.record R) v)).
+    Variable (prelval : ∀ (rv : RelVal (ty.record R)), P (term_relval (ty.record R) rv)).
+    Variable (precord : ∀ (ts : NamedEnv (Term Σ) (recordf_ty R)), P (term_record R ts)).
 
-    (* Equations(noeqns) Term_record_case (t : Term Σ (ty.record R)) : P t := *)
-    (* | term_var_in lIn => pvar lIn *)
-    (* | term_val _ v    => pval v *)
-    (* | term_record ts  => precord ts. *)
+    Equations(noeqns) Term_record_case (t : Term Σ (ty.record R)) : P t :=
+    | term_var_in lIn => pvar lIn
+    | term_val _ v    => pval v
+    | term_relval _ rv    => prelval rv
+    | term_record ts  => precord ts.
 
   End Term_record_case.
 
@@ -556,42 +564,44 @@ Module Type TermsOn (Import TY : Types).
     Local Set Elimination Schemes.
 
     (* A view on list terms. *)
-    (* Inductive ListView {Σ σ} : Term Σ (ty.list σ) → Type := *)
-    (* | term_list_var {ς} {ςInΣ : (ς∷ty.list σ) ∈ Σ} : *)
-    (*   ListView (term_var ς) *)
-    (* | term_list_val v : *)
-    (*   ListView (term_val _ v) *)
-    (* | term_list_cons h {t} (lv : ListView t) : *)
-    (*   ListView (term_binop bop.cons h t) *)
-    (* | term_list_append {t1 t2} (lv1 : ListView t1) (lv2 : ListView t2) : *)
-    (*   ListView (term_binop bop.append t1 t2) *)
-    (* | term_list_rev t (lv : ListView t) : *)
-    (*   ListView (term_unop uop.rev t). *)
-    (* #[global] Arguments term_list_var {Σ σ} ς {ςInΣ}. *)
-    (* #[global] Arguments term_list_append {Σ σ} [t1 t2] lv1 lv2. *)
+    Inductive ListView {Σ σ} : Term Σ (ty.list σ) → Type :=
+    | term_list_var {ς} {ςInΣ : (ς∷ty.list σ) ∈ Σ} :
+      ListView (term_var ς)
+    | term_list_val v :
+      ListView (term_val _ v)
+    | term_list_relval v :
+      ListView (term_relval _ v)
+    | term_list_cons h {t} (lv : ListView t) :
+      ListView (term_binop bop.cons h t)
+    | term_list_append {t1 t2} (lv1 : ListView t1) (lv2 : ListView t2) :
+      ListView (term_binop bop.append t1 t2)
+    | term_list_rev t (lv : ListView t) :
+      ListView (term_unop uop.rev t).
+    #[global] Arguments term_list_var {Σ σ} ς {ςInΣ}.
+    #[global] Arguments term_list_append {Σ σ} [t1 t2] lv1 lv2.
 
     (* We map each type to a specialized view for that type. *)
     Definition View {Σ} (σ : Ty) : Term Σ σ → Type :=
       match σ with
-      (* | ty.list τ => ListView *)
+      | ty.list τ => ListView
       | _         => fun _ => unit
       end.
 
     Definition view_var {Σ l σ} : ∀ lIn, View (@term_var Σ l σ lIn) :=
       match σ with
-       (* | ty.list σ => @term_list_var _ _ l *)
+       | ty.list σ => @term_list_var _ _ l
        | _         => fun _ => tt
        end.
 
     Definition view_val {Σ σ} : ∀ v, View (@term_val Σ σ v) :=
       match σ with
-      (* | ty.list σ0 => term_list_val *)
+      | ty.list σ0 => term_list_val
       | _          => fun _ => tt
       end.
 
     Definition view_relval {Σ σ} : ∀ v, View (@term_relval Σ σ v) :=
       match σ with
-      (* | ty.list σ0 => term_list_val *)
+      | ty.list σ0 => term_list_relval
       | _          => fun _ => tt
       end.
 
@@ -599,15 +609,15 @@ Module Type TermsOn (Import TY : Types).
       ∀ {t1 : Term Σ σ1} {t2 : Term Σ σ2},
         View t1 → View t2 → View (term_binop op t1 t2) :=
        match op with
-       (* | bop.cons   => fun t1 t2 _  v2 => term_list_cons t1 v2 *)
-       (* | bop.append => term_list_append *)
+       | bop.cons   => fun t1 t2 _  v2 => term_list_cons t1 v2
+       | bop.append => term_list_append
        | _ => fun _ _ _ _ => tt
        end.
 
     Definition view_unop {Σ σ1 σ2} (op : UnOp σ1 σ2) :
       ∀ {t : Term Σ σ1}, View t → View (term_unop op t) :=
     match op with
-      (* | uop.rev => term_list_rev *)
+      | uop.rev => term_list_rev
       | _ => fun _ _ => tt
       end.
 
@@ -648,16 +658,16 @@ Module Type TermsOn (Import TY : Types).
           Term_eqb t1 t2;
         Term_eqb (term_unop op1 t1) (term_unop op2 t2) (right _) := false;
       };
-      (* Term_eqb (@term_tuple ?(σs) xs) (@term_tuple σs ys) := *)
-      (*   @env.eqb_hom _ (Term Σ) Term_eqb _ xs ys; *)
+      Term_eqb (@term_tuple ?(σs) xs) (@term_tuple σs ys) :=
+        @env.eqb_hom _ (Term Σ) Term_eqb _ xs ys;
       Term_eqb (@term_union ?(u) _ k1 e1) (@term_union u _ k2 e2)
         with eq_dec k1 k2 => {
         Term_eqb (term_union k1 e1) (term_union ?(k1) e2) (left eq_refl) :=
           Term_eqb e1 e2;
         Term_eqb _ _ (right _) := false
       };
-      (* Term_eqb (@term_record ?(r) xs) (@term_record r ys) := *)
-      (*   @env.eqb_hom _ (fun b => Term Σ (type b)) (fun b => @Term_eqb (type b)) _ xs ys; *)
+      Term_eqb (@term_record ?(r) xs) (@term_record r ys) :=
+        @env.eqb_hom _ (fun b => Term Σ (type b)) (fun b => @Term_eqb (type b)) _ xs ys;
       Term_eqb _ _ := false
     .
 
@@ -679,12 +689,12 @@ Module Type TermsOn (Import TY : Types).
                 destruct (uop.tel_eq_dec x y) as [e|];
                 [dependent elimination e|]
             | H: ~ bop.OpEq ?o ?o |- False => apply H; constructor
-            (* | |- reflect (term_tuple ?ts1 = term_tuple ?ts2) _ => *)
-            (*     apply (@ssrbool.iffP (ts1 = ts2)) *)
-            (* | |- reflect (term_record ?R ?ts1 = term_record ?R ?ts2) _ => *)
-            (*     apply (@ssrbool.iffP (ts1 = ts2)) *)
-            (* | |- reflect (?ts1 = ?ts2) (env.eqb_hom _ ?ts1 ?ts2) => *)
-            (*     apply env.eqb_hom_spec_point *)
+            | |- reflect (term_tuple ?ts1 = term_tuple ?ts2) _ =>
+                apply (@ssrbool.iffP (ts1 = ts2))
+            | |- reflect (term_record ?R ?ts1 = term_record ?R ?ts2) _ =>
+                apply (@ssrbool.iffP (ts1 = ts2))
+            | |- reflect (?ts1 = ?ts2) (env.eqb_hom _ ?ts1 ?ts2) =>
+                apply env.eqb_hom_spec_point
             end; auto.
     Qed.
 
@@ -716,9 +726,9 @@ Module Type TermsOn (Import TY : Types).
       | term_relval σ v               => term_relval σ v
       | term_binop op t1 t2        => term_binop op (sub_term t1 ζ) (sub_term t2 ζ)
       | term_unop op t             => term_unop op (sub_term t ζ)
-      (* | term_tuple ts              => term_tuple (env.map (fun _ t => sub_term t ζ) ts) *)
+      | term_tuple ts              => term_tuple (env.map (fun _ t => sub_term t ζ) ts)
       | term_union U K t           => term_union U K (sub_term t ζ)
-      (* | term_record R ts           => term_record R (env.map (fun _ t => sub_term t ζ) ts) *)
+      | term_record R ts           => term_record R (env.map (fun _ t => sub_term t ζ) ts)
       end.
 
     #[export] Instance SubstTerm {σ} : Subst (fun Σ => Term Σ σ) :=
@@ -802,14 +812,14 @@ Module Type TermsOn (Import TY : Types).
       { intros ? t.
         induction t; cbn; f_equal; try assumption.
         - unfold sub_id. now rewrite env.lookup_tabulate.
-        (* - induction IH; cbn; f_equal; auto. *)
-        (* - induction IH; cbn; f_equal; auto. *)
+        - induction IH; cbn; f_equal; auto.
+        - induction IH; cbn; f_equal; auto.
       }
       { intros ? ? ? ? ? t.
         induction t; cbn; f_equal; try assumption.
         - unfold subst at 1, SubstEnv. now rewrite env.lookup_map.
-        (* - induction IH; cbn; f_equal; auto. *)
-        (* - induction IH; cbn; f_equal; auto. *)
+        - induction IH; cbn; f_equal; auto.
+        - induction IH; cbn; f_equal; auto.
       }
     Qed.
 
@@ -1090,8 +1100,8 @@ Module Type TermsOn (Import TY : Types).
     Notation "e1 - e2" := (term_minus e1 e2) : term_scope.
     Notation "e1 && e2" := (term_and e1 e2) : term_scope.
     Notation "e1 || e2" := (term_or e1 e2) : term_scope.
-    (* Notation "e1 :: e2" := (term_cons e1 e2) : term_scope. *)
-    (* Notation "e1 ++ e2" := (term_append e1 e2) : term_scope. *)
+    Notation "e1 :: e2" := (term_cons e1 e2) : term_scope.
+    Notation "e1 ++ e2" := (term_append e1 e2) : term_scope.
     Notation "e1 +ᵇ e2" := (term_bvadd e1 e2) : term_scope.
     Notation "e1 -ᵇ e2" := (term_bvsub e1 e2) : term_scope.
     Notation "e1 *ᵇ e2" := (term_bvmul e1 e2) : term_scope.
